compiler/eval/compilerComputeLib.sml
@@ -331,6 +331,7 @@ val add_compiler_compset = computeLib.extend_compset
     ,bvp_to_wordTheory.shift_def
     ,bvp_to_wordTheory.StoreEach_def
     ,bvp_to_wordTheory.shift_length_def
+    ,bvp_to_wordTheory.max_heap_limit_def
     ,bvp_to_wordTheory.real_addr_def
     ,bvp_to_wordTheory.real_offset_def
     ,bvp_to_wordTheory.all_ones_def
